Foam.lean
@@ -91,4 +91,5 @@ import Foam.Bridges.Nicaea
 import Foam.Bridges.Grover
 import Foam.Bridges.Narayana
 import Foam.Bridges.Leibniz
+import Foam.Bridges.Fraenkel
 import Foam.Bridges.Hofstadter
